Isabelle2/AbstractMultiPaxosR2Correctness.thy
@@ -1,0 +1,83 @@
+theory AbstractMultiPaxosR2Correctness
+imports AbstractMultiPaxosR1 AbstractMultiPaxosR2 "../IO-Automata/Simulations"
+begin
+
+print_locale ampr2_ioa
+
+locale ampr2_proof = IOA + quorums quorums + ampr2_ioa quorums for
+     quorums :: "'a set set" +
+  fixes ampr2_ioa :: "(('v,'a,'l)ampr2_state, ('v,'a,'l)ampr1.amp_action) ioa"
+  and ampr1_ioa :: "(('v,'a,'l)amp_state, ('v,'a,'l)ampr1.amp_action) ioa"
+  defines "ampr2_ioa \<equiv> ioa" and "ampr1_ioa \<equiv> ampr1.amp_ioa"
+begin
+
+definition ref_map :: "('v,'a,'l)ampr2_state \<Rightarrow> ('v,'a,'l)amp_state" where 
+  "ref_map s \<equiv> \<lparr> amp_state.propCmd = (propCmd s),
+  ballot = (\<lambda>a. ((ballot s) $ a)),
+  vote = (\<lambda>a i b. (vote s $ a $ i $ b)),
+  suggestion = (\<lambda>i b. ((suggestion s i) $ b)),
+  onebs = (\<lambda>a b. (onebs s $ a $ b)),
+  learned = (\<lambda>l i. (learned s $ l $ i)),
+  leader = (\<lambda>a. (ampr2_state.leader s $ a)) \<rparr>"
+
+term "ampr1_ioa"
+term "ampr2_ioa"
+
+lemma "is_ref_map ref_map ampr2_ioa ampr1_ioa"
+proof (auto simp add:is_ref_map_def simp del:split_paired_Ex)
+  fix s
+  assume "s \<in> ioa.start ampr2_ioa"
+  thus "ref_map s \<in> ioa.start ampr1_ioa" 
+    apply (simp add:ref_map_def ampr1.simps ampr2_ioa_def ampr1_ioa_def ioa_def start_def)
+next
+  fix s t a
+  assume a1:"reachable ampr2_ioa s" and a2:"s \<midarrow>a\<midarrow>ampr2_ioa\<longrightarrow> t"
+  let ?e = "(ref_map s, [(a, ref_map t)])"
+  have "refines ?e s a t ampr1_ioa ref_map"
+  proof (auto simp add:refines_def ioa_simps trace_match_def trace_def schedule_def filter_act_def)
+    show "(ref_map s, a, ref_map t) \<in> ioa.trans ampr1_ioa" using a2
+    apply (simp add:ampr2_ioa_def ioa_def is_trans_def trans_def)
+    apply (simp add:ampr1_ioa_def ampr1.ioa_def ampr1.trans_def)
+    apply (induct rule:trans_cases_2)
+    apply (simp_all add:simps ampr1.simps ref_map_def)[2]
+    (* join_ballot *)
+    apply (induct a) apply auto[2]
+    apply (auto simp add:ref_map_def ampr1.simps simps)[1]
+    (* do_vote *)
+    apply (induct a) apply auto[2] 
+    subgoal premises prems for a i v
+    proof -
+      have "ampr1.do_vote a i v (ref_map s) (ref_map t)" using prems
+        by (auto simp add:ref_map_def simps Let_def ampr1.simps fun_eq_iff)
+      thus ?thesis by auto
+    qed
+    (* suggest *)
+    apply (induct a) apply auto[2] 
+    subgoal premises prems for a i b v
+    proof -
+      have "ampr1.suggest a i b v (ref_map s) (ref_map t)" using prems
+        by (auto simp add:ref_map_def simps Let_def ampr1.simps fun_eq_iff)
+      thus ?thesis by auto
+    qed
+    (* catch_up *)
+    apply (induct a) apply auto[2] 
+    subgoal premises prems for l1 l2 i v
+    proof -
+      have "ampr1.catch_up l1 l2 i v (ref_map s) (ref_map t)" using prems
+        by (auto simp add:ref_map_def simps Let_def ampr1.simps fun_eq_iff)
+      thus ?thesis by auto
+    qed
+    (* acquire_leadership *)
+    apply (induct a) apply auto[2] 
+    subgoal premises prems for aa q
+    proof -
+      have "ampr1.acquire_leadership aa q (ref_map s) (ref_map t)" using prems
+        by (auto simp add:ref_map_def simps Let_def ampr1.simps fun_eq_iff)
+      thus ?thesis by auto
+    qed
+    done 
+    qed
+  thus "\<exists> e . refines e s a t ampr1_ioa ref_map" by blast
+qed
+
+end
